src/algebras/dill.v
@@ -1,4 +1,5 @@
 From Hammer Require Import Hammer.
+From Coq.Logic Require Import FunctionalExtensionality PropExtensionality.
 From VST.msl Require Import sepalg sepalg_generators.
 From CARVe.algebras Require Import linear structural.
 
@@ -12,9 +13,43 @@ Definition omega : mult := inr tt.
 Instance Join_mult : Join mult :=
   Join_sum _ linear.Join_mult _ structural.Join_mult.
 
+Variant hal : mult -> Prop :=
+  | halz : hal zero
+  | halo : hal omega.
+
+Property hal_is_identity : hal = identity.
+Proof.
+  extensionality x; apply propositional_extensionality; split; intro H.
+  - inversion H; intros ? ? ?; sauto.
+  - destruct x as [lx | sx].
+    + destruct lx.
+      * constructor.
+      * assert (H' : join one zero one) by constructor; discriminate (H _ _ H').
+    + destruct sx; constructor.
+Qed.
+
+Definition hal_core : mult -> Prop := fun m => m = core m.
+
+Property hal_is_core : hal = hal_core.
+Proof. extensionality x; apply propositional_extensionality; sauto. Qed.
+
+Property join_hal {x y z : mult} :
+  join x y z -> hal z -> x = z.
+Proof. intros; destruct H0; destruct x, y; inversion H; sauto. Qed.
+
+(* Useful characterization property *)
+Property join_cases {x y z : mult} :
+  join x y z ->
+  match z with
+  | inl linear.zero => x = zero /\ y = zero
+  | inl linear.one => (x = one /\ y = zero) \/ (x = zero /\ y = one)
+  | inr tt => x = omega /\ y = omega
+  end.
+Proof. destruct x, y, z; sauto. Qed.
+
 (* The following definition and lemma are an inductive
-characterization of the join that MSL generates. They exists solely to
-reassure the reader that the framework does the right thing, and they
+characterization of the join that MSL generates. These exists solely to
+reassure the reader that the framework does the 'right thing'; they
 are not meant to be used in proof developments. *)
 
 Inductive mult_op : mult -> mult -> mult -> Prop:=
@@ -23,9 +58,11 @@ Inductive mult_op : mult -> mult -> mult -> Prop:=
 | m_01 : mult_op zero one one
 | m_ωω : mult_op omega omega omega.
 
-Lemma join_is_mult_op : forall (x y z : mult),
-    join x y z <-> mult_op x y z.
+Property join_is_mult_op : forall (x y z : mult),
+  join x y z <-> mult_op x y z.
 Proof. sauto. Qed.
+
+(* Proving mult is a separation algebra *)
 
 Instance mult_Perm_alg : Perm_alg mult :=
   Perm_sum _ _ _ _ linear.Perm_alg_mult structural.Perm_mult.
@@ -33,11 +70,5 @@ Instance mult_Perm_alg : Perm_alg mult :=
 Instance mult_Sep_alg : Sep_alg mult :=
   Sep_sum _ _ _ _ _ _ linear.mult_Sep_alg structural.Sep_mult.
 
-Variant hal : mult -> Prop :=
-  | halz : hal zero
-  | halo : hal omega.
-
-Definition hal_core : mult -> Prop := fun m => m = (core m).
-
-Lemma hal_is_core : forall x, hal x <-> hal_core x.
-Proof. sauto. Qed.
+Instance mult_Flat_alg : Flat_alg mult.
+Proof. constructor; intros. rewrite join_is_mult_op in H; destruct H; constructor. Defined.
