src/algebras/structural.v
@@ -5,13 +5,15 @@ From VST.msl Require Import sepalg sepalg_generators.
 
 Definition mult : Type := unit.
 
-  Variant hal : mult -> Prop :=
+Variant hal : mult -> Prop :=
   | halo : hal tt.
 
-  Instance Join_mult : Join mult := Join_unit.
-  Instance Canc_mult : Canc_alg mult := Canc_unit.
-  Instance Perm_mult : Perm_alg mult := Perm_unit.
-  Instance Sep_mult : Sep_alg mult.
-  exists (fun _ => tt); auto with *.
+Instance Join_mult : Join mult := Join_unit.
+Instance Canc_mult : Canc_alg mult := Canc_unit.
+Instance Perm_mult : Perm_alg mult := Perm_unit.
 
-Defined.
+Instance Sep_mult : Sep_alg mult.
+Proof. exists (fun _ => tt); auto with *. Defined.
+
+Instance Flat_mult : Flat_alg mult.
+Proof. constructor. intros []. reflexivity. Defined.
