case_studies/closures/README.md
@@ -7,10 +7,10 @@ The operational semantics is big-step and does not perform substitutions, so no 
 
 ## Files
 
-- **ndbclo.v**:  
-  Numbered (but not well-scoped) DB encoding. 
+- **ndbclo.v**:
+  Numbered (but not well-scoped) DB encoding.
   Includes proofs of subject reduction and weak normalization.
 
-- **basicIclo.v**:  
-  Intrinsically-typed DB version, but **not** linear. 
+- **basicIclo.v**:
+  Intrinsically-typed DB version, but **not** linear.
   Meant as a stepping stone toward a future fully linear version.
